theories/iris_fundamental.v
@@ -1,0 +1,146 @@
+From mathcomp Require Import ssreflect eqtype seq ssrbool.
+From iris.program_logic Require Import language.
+From iris.proofmode Require Import base tactics classes.
+From iris.base_logic Require Export gen_heap ghost_map proph_map na_invariants.
+From iris.base_logic.lib Require Export fancy_updates.
+From iris.algebra Require Import list.
+From iris.prelude Require Import options.
+
+Require Export iris iris_locations iris_properties iris_atomicity stdpp_aux.
+Require Export iris_rules.
+Require Export datatypes host operations properties opsem typing.
+Require Export iris_logrel.
+Import uPred.
+
+Section fundamental.
+  Import DummyHosts. (* placeholder *)
+
+  Context `{!wfuncG Σ, !wtabG Σ, !wmemG Σ, !wmemsizeG Σ, !wglobG Σ, !wframeG Σ, HWP: host_program_logic, !logrel_na_invs Σ}.
+
+  Ltac take_drop_app_rewrite n :=
+    match goal with
+    | |- context [ WP ?e @ _; _ CTX _; _ {{ _ }} %I ] =>
+        rewrite -(list.take_drop n e);simpl take; simpl drop
+    | |- context [ WP ?e @ _; _ {{ _ }} %I ] =>
+        rewrite -(list.take_drop n e);simpl take; simpl drop
+    | |- context [ WP ?e @ _; _ FRAME _; _ CTX _; _  {{ _, _ }} %I ] =>
+        rewrite -(list.take_drop n e);simpl take; simpl drop
+    | |- context [ WP ?e @ _; _ FRAME _; _ {{ _ }} %I ] =>
+        rewrite -(list.take_drop n e);simpl take; simpl drop
+    end.
+  
+  Ltac take_drop_app_rewrite_twice n m :=
+    take_drop_app_rewrite n;
+    match goal with
+    | |- context [ WP _ ++ ?e @ _; _ CTX _; _ {{ _ }} %I ] =>
+        rewrite -(list.take_drop (length e - m) e);simpl take; simpl drop
+    | |- context [ WP _ ++ ?e @ _; _ {{ _ }} %I ] =>
+        rewrite -(list.take_drop (length e - m) e);simpl take; simpl drop
+    end.
+
+  Lemma interp_value_type_of v : (⊢ interp_value (Σ:=Σ) (typeof v) v)%I.
+  Proof.
+    unfold interp_value.
+    destruct v;simpl;eauto.
+  Qed.
+    
+  Theorem be_fundamental C es τ : be_typing C es τ -> ⊢ semantic_typing (HWP:=HWP) C (to_e_list es) τ.
+  Proof.
+    induction 1.
+    
+    {
+      unfold semantic_typing, interp_expression.
+      iIntros (i lh f vs).
+      destruct C,i.
+      iIntros "(#Hi & Hf & %Hlh) #Hv".
+      iDestruct "Hf" as (locs Heq) "[#Hlocs Hf]".
+      iDestruct "Hv" as "[-> | Hv]".
+      { take_drop_app_rewrite_twice 0 1.
+        iApply (wp_wand_r _ _ _ (λ vs, interp_val [typeof v] vs ∗  ↪[frame]f)%I). iSplitL.
+        { iApply (wp_trap with "[] [$]");auto. by iLeft. }
+        iIntros (v0) "[? ?]". iFrame. iExists _. iFrame. }
+      { iDestruct "Hv" as (ws ->) "Hv".
+        iDestruct (big_sepL2_nil_inv_r with "Hv") as %->.
+        iApply (wp_wand_r _ _ _ (λ vs, interp_val [typeof v] vs ∗  ↪[frame]f)%I). iSplitL.
+        { rewrite app_nil_l.
+          iApply wp_value;[by instantiate (1:= immV [_])|].
+          iFrame. iRight. iExists _. iSplit;eauto.
+          iSimpl; iSplit =>//. iApply interp_value_type_of. }
+        iIntros (v0) "[? ?]". iFrame. iExists _. iFrame. 
+      }
+    }
+
+
+    12: {
+      unfold semantic_typing, interp_expression.
+      iIntros (i lh f vs).
+      destruct C,i.
+      set (C := {|
+                 tc_types_t := tc_types_t;
+                 tc_func_t := tc_func_t;
+                 tc_global := tc_global;
+                 tc_table := tc_table;
+                 tc_memory := tc_memory;
+                 tc_local := tc_local;
+                 tc_label := tc_label;
+                 tc_return := tc_return
+               |}
+          ).
+      set (i := {|
+                 inst_types := inst_types;
+                 inst_funcs := inst_funcs;
+                 inst_tab := inst_tab;
+                 inst_memory := inst_memory;
+                 inst_globs := inst_globs
+               |}).
+      iIntros "(#Hi & Hf & %Hlh) #Hv".
+      iDestruct "Hv" as "[-> | Hv]".
+      { iDestruct "Hf" as (locs Heq) "[#Hlocs Hf]". 
+        take_drop_app_rewrite_twice 0 1.
+        iApply (wp_wand_r _ _ _ (λ vs, interp_val tm vs ∗  ↪[frame]f)%I). iSplitL.
+        { iApply (wp_trap with "[] [$]");auto. by iLeft. }
+        iIntros (v0) "[? ?]". iFrame. iExists _. iFrame. }
+      iDestruct "Hv" as (ws ->) "Hv".
+      iDestruct (big_sepL2_length with "Hv") as %Hlen.
+      iDestruct "Hf" as (locs Heq) "[#Hlocs Hf]".
+      iApply (wp_loop with "Hf");eauto.
+      { apply v_to_e_is_const_list. }
+      { rewrite fmap_length //. }
+      iNext. iIntros "Hf".
+      iDestruct (IHbe_typing with "[Hf] []") as "HH".
+      { iFrame "# ∗". unfold interp_ctx. simpl. instantiate (1:=LH_rec (of_val (immV ws)) (length tn) _ lh _).
+        iSplit;[iExists _;eauto|].
+        iPureIntro. destruct Hlh as [Hbase Hlenh]. auto. }
+      { instantiate (1:=immV ws). iRight. eauto. }
+      iApply wp_wasm_empty_ctx.
+      iApply wp_label_push_nil. iSimpl.
+      unfold interp_expression,interp_val.
+      iAssert (WP of_val (immV ws) ++ to_e_list es
+                  {{ vs, ⌜vs = trapV⌝ ∗ (∃ f0 : leibnizO frame,  ↪[frame]f0) }} ∨
+              WP of_val (immV ws) ++ to_e_list es
+                 {{ vs, (∃ ws0 : seq.seq (leibnizO value), ⌜vs = immV ws0⌝ ∗ ([∗ list] w;τ ∈ ws0;tm, interp_value τ w))
+                          ∗ (∃ f0 : leibnizO frame,  ↪[frame]f0) }})%I with "[HH]" as "HHH".
+      { }
+
+      
+      iApply wp_seq_ctx.
+
+      iDestruct "HH" as (f0) "HH". iExists f0.
+      
+
+
+      
+      iDestruct (IHbe_typing with "[Hf] []") as "HH".
+      { iFrame "# ∗". unfold interp_ctx. simpl. instantiate (1:=LH_rec (of_val (immV ws)) (length tn) _ lh _).
+        iPureIntro. destruct Hlh as [Hbase Hlen]. auto. }
+      { instantiate (1:=immV ws). iRight. eauto. }
+      iDestruct "HH" as (f0) "HH". iExists f0.
+      iDestruct (big_sepL2_length with "Hv") as %Hlen.
+      iApply wp_loop;eauto.
+      { apply v_to_e_is_const_list. }
+      { rewrite fmap_length //. }
+      { eauto. } apply const_list_of_val.
+     
+
+
+End fundamental.
