theories/iris_rules_trap.v
@@ -3,7 +3,7 @@ From iris.program_logic Require Import language.
 From iris.proofmode Require Import base tactics classes.
 From iris.base_logic Require Export gen_heap ghost_map proph_map.
 From iris.base_logic.lib Require Export fancy_updates.
-Require Export datatypes host operations properties opsem.
+Require Export datatypes host operations properties opsem iris_rules_control.
 Require Export iris_wp_def stdpp_aux.
 
 
@@ -148,7 +148,7 @@ Section trap_rules.
         destruct σ2 as [[[??] ?]?].
         iDestruct "H2" as "[Hσ H]".
         iDestruct "H" as (f1) "(Hf1 & Hes'' & Hefs)".
-        iExists f1.
+        iApply bi.sep_exist_l. iExists f1.
         iFrame. (* iSplit =>//. *)
         iIntros "?".
         iSpecialize ("IH" with "[$]").
@@ -188,5 +188,443 @@ Section trap_rules.
         iApply wp_trap;auto. }
   Qed.
 
+  Lemma wp_val_trap (s : stuckness) (E : coPset) v0 (es1 : language.expr wasm_lang) f f' :
+    ↪[frame] f ∗
+     (↪[frame] f -∗ WP es1 @ NotStuck; E {{ w, ⌜w = trapV⌝ ∗ ↪[frame] f' }})
+     ⊢ WP ((AI_basic (BI_const v0)) :: es1) @ s; E {{ w, ⌜w = trapV⌝ ∗ ↪[frame] f' }}.
+  Proof.
+  (* This also needs an iLob. *)
+  iLöb as "IH" forall (v0 es1 f f').
+  iIntros "(Hntrap & H)".
+  (* iApply wp_unfold.                *)
+  destruct (iris.to_val es1) as [vs|] eqn:Hes.
+  { repeat rewrite wp_unfold /wp_pre /= Hes.
+    iMod ("H"  with "Hntrap") as "[%Hcontr Hf]". subst.
+    apply to_val_trap_is_singleton in Hes as ->.
+    rewrite -(app_nil_r [AI_trap]). rewrite separate1.
+    iApply (wp_trap with "[] [Hf]");auto. }
+  { repeat rewrite wp_unfold /wp_pre /= Hes.
+    iApply wp_unfold. rewrite /wp_pre /=.
+    rewrite Hes. 
+    iIntros (?????) "?".
+    iDestruct ("H" with "[$]") as "H".
+    iSpecialize ("H" $! σ1 ns κ κs nt with "[$]").
+    iMod "H" as "[%Hred H]".
+    iModIntro.
+    iSplit.
+    { iPureIntro.
+      destruct s =>//. rewrite separate1.
+      eapply prepend_reducible;eauto. }
+    iIntros (es2 σ2 efs HStep).
+    rewrite separate1 in HStep.
+    apply prim_step_obs_efs_empty in HStep as Heq. simplify_eq.
+    apply reduce_ves in HStep as [[-> Hstep] | [lh [lh' [Hfill1 [Hfill2 ->]]]]].
+    { iSpecialize ("H" $! _ _ _ Hstep).
+      repeat (iMod "H"; iModIntro; try iNext).
+      iDestruct "H" as "[$ Ha]".
+      iDestruct "Ha" as (a) "[Hf [Ha _]]".
+      iExists _. iFrame. simpl.
+      iSplit =>//. iIntros "Hf".
+      iApply "IH". iFrame. }
+    { apply lfilled_Ind_Equivalent in Hfill1.
+      apply lfilled_Ind_Equivalent in Hfill2.
+      inversion Hfill1;inversion Hfill2;simplify_eq.
+      assert (iris.prim_step (vs0 ++ [AI_trap] ++ es'0)%SEQ σ2 [] [AI_trap] σ2 []) as Hstep'.
+      { destruct σ2 as [[[??] ?]?]. split =>//.
+        apply r_simple; eapply rs_trap => //.
+        2: apply lfilled_Ind_Equivalent;constructor=>//.
+        destruct vs0;[|destruct vs0 =>//].
+        destruct es'0;[|destruct es'0 =>//].
+        erewrite app_nil_l, app_nil_r in Hes. done.
+      }
+      iSpecialize ("H" $! _ _ _ Hstep').
+      repeat (iMod "H"; iModIntro; try iNext).
+      iDestruct "H" as "[$ Ha]".
+      iDestruct "Ha" as (a) "[Hf [Ha _]]".
+      iExists _. iFrame. simpl.
+      iSplit =>//. iIntros "Hf".
+      iDestruct ("Ha" with "Hf") as "Ha".
+      rewrite wp_unfold /wp_pre /=.
+      iMod "Ha" as "[_ Hf]".
+      erewrite cons_middle.
+      iApply wp_trap;auto. } 
+    auto.
+  }
+  Qed.
+      
+  Lemma wp_val_app_trap' (s : stuckness) (E : coPset) vs (es : language.expr wasm_lang) f f' :
+    ↪[frame] f ∗
+     (↪[frame] f -∗ WP es @ NotStuck ; E {{ w, ⌜w = trapV⌝ ∗ ↪[frame] f' }}%I)
+     ⊢ WP ((v_to_e_list vs) ++ es) @ s ; E {{ w, ⌜w = trapV⌝ ∗ ↪[frame] f' }}%I.
+  Proof.
+    iInduction vs as [|c vs] "IH" forall (s E es).
+    { simpl.
+      iIntros "[Hf HWP]".
+      destruct s.
+      2: iApply wp_stuck_weaken.
+      all: iDestruct ("HWP" with "Hf") as "HWP".
+      all: iApply (wp_wand with "HWP").
+      all: iIntros (v).
+      all: destruct v => /=.
+      all: iIntros "HΦ" => //.
+    }
+    { iIntros "[Hf HWP]".
+      iSimpl.
+      iApply wp_val_trap.
+      iFrame. iIntros "Hf".
+      iApply ("IH" $! _ _ _ with "[Hf HWP]") => //=.
+      iFrame.
+    }
+  Qed.
+  
+  Lemma wp_val_app_trap (s : stuckness) (E : coPset) vs v' (es : language.expr wasm_lang) f f' :
+    iris.to_val vs = Some (immV v') ->
+    ↪[frame] f ∗
+     (↪[frame] f -∗ WP es @ NotStuck ; E {{ w, ⌜w = trapV⌝ ∗ ↪[frame] f'}}%I)
+     ⊢ WP (vs ++ es) @ s ; E {{ w, ⌜w = trapV⌝ ∗ ↪[frame] f' }}%I.
+  Proof.
+    iIntros "%Hves [Hf Hwp]".
+    apply iris.of_to_val in Hves; subst.
+    iApply wp_val_app_trap'.
+    by iFrame.
+  Qed.
+
+  Lemma wp_label_trap s E LI vs n es' es'' f f':
+    const_list vs ->
+    ↪[frame] f -∗
+    (↪[frame] f -∗ WP LI @ E {{ w, ⌜w = trapV⌝ ∗  ↪[frame]f' }}) -∗
+    WP vs ++ [AI_label n es' LI] ++ es'' @ s; E {{ w, ⌜w = trapV⌝ ∗  ↪[frame]f' }}.
+  Proof.
+    iLöb as "IH" forall (vs LI es' f f' es'' s).
+    iIntros (Hconst) "Hf Hcont".
+    destruct (iris.to_val LI) eqn:He.
+    { iDestruct ("Hcont" with "Hf") as "Hcont".
+      iDestruct (wp_unfold with "Hcont") as "Hcont".
+      rewrite /wp_pre /= He.
+      iMod "Hcont" as "[%Hcontr Hf]". subst.
+      apply to_val_trap_is_singleton in He as ->.
+      apply const_list_is_val in Hconst as [v Hv].
+      iApply wp_val_app_trap;eauto. iFrame.
+      iIntros "Hf".
+      rewrite separate1.
+      iApply wp_seq_trap. iFrame. iIntros "Hf".
+      iApply (wp_label_trap with "Hf");auto. }
+    { apply const_list_is_val in Hconst as [v Hv].
+      iApply wp_val_app_trap;eauto. iFrame.
+      iIntros "Hf".
+      iApply wp_seq_trap. iFrame. iIntros "Hf".
+      iDestruct ("Hcont" with "Hf") as "Hcont".
+      iDestruct (wp_unfold with "Hcont") as "Hcont".
+      iApply wp_unfold.
+      rewrite /wp_pre /= He.
+      iIntros (σ ns κ κs nt) "Hσ".
+      iSpecialize ("Hcont" $! σ 0 [] [] 0).
+      iDestruct ("Hcont" with "[$]") as "H".
+      iMod "H" as "[%Hred H]".
+      iModIntro.
+      assert (lfilled 1 (LH_rec [] n es' (LH_base [] []) []) (LI ++ []) [AI_label n es' LI]) as Hfill.
+      { apply lfilled_Ind_Equivalent.
+        rewrite -(app_nil_l [AI_label n es' LI]) -(app_nil_r [AI_label n es' LI]).
+        constructor=>//.
+        apply lfilled_Ind_Equivalent. cbn. erewrite app_nil_r, app_nil_r. by rewrite eqseqE. }
+      iSplit.
+      { iPureIntro.
+        unfold iris_wp_def.reducible, reducible.
+        destruct Hred as [? [? [? [? ?]]]].
+        exists [], [AI_label n es' x0],x1,[].
+        destruct x1 as [[[? ?] ?] ?].
+        destruct σ as [[[? ?] ?] ?].
+        split =>//.
+        eapply r_label. apply H.
+        erewrite app_nil_r in Hfill. apply Hfill.
+        apply lfilled_Ind_Equivalent.
+        rewrite -(app_nil_l [AI_label n es' x0]) -(app_nil_r [AI_label n es' x0]).
+        constructor=>//.
+        apply lfilled_Ind_Equivalent. cbn. by rewrite eqseqE app_nil_r. }
+      iIntros (e2 σ2 efs Hstep).
+      apply prim_step_obs_efs_empty in Hstep as Heq. simplify_eq.
+      eapply lfilled_prim_step_split_reduce_r in Hstep;[|eauto|auto].
+      destruct Hstep as [[e' [Hstep Hfill']]|[[lh Hfill'] ->]].
+      { apply lfilled_Ind_Equivalent in Hfill'. inversion Hfill';subst.
+        inversion H8;simplify_eq.
+        apply prim_step_obs_efs_empty in Hstep as Heq;simplify_eq.
+        iSpecialize ("H" $! _ _ _ Hstep).
+        repeat (iMod "H"; iModIntro; try iNext).
+        destruct σ2 as [[[? ?]?]?].
+        iDestruct ("H") as "[$ H]".
+        iDestruct "H" as (f0) "[Hf [H _]]".
+        iExists f0. iFrame.
+        iSplit =>//. iIntros "Hf".
+        repeat erewrite app_nil_r,app_nil_l. erewrite app_nil_r.
+        iDestruct ("IH" $! [] _ es' _ _ [] with "[] Hf H") as "H";auto. }
+      {
+        apply lfilled_Ind_Equivalent in Hfill'.
+        inversion Hfill';subst.
+        assert (iris.prim_step (vs0 ++ [AI_trap] ++ es'0)%SEQ σ2 [] [AI_trap] σ2 []) as Hstep'.
+        { destruct σ2 as [[[? ?] ?] ?].
+          split =>//.
+          eapply r_simple,rs_trap.
+          2: instantiate (1 := LH_base vs0 es'0);apply lfilled_Ind_Equivalent;by constructor.
+          destruct vs0,es'0 =>//; destruct vs0 =>//. }
+        iSpecialize ("H" $! _ _ _ Hstep').
+        repeat (iMod "H"; iModIntro; try iNext).
+        iDestruct "H" as "[$ H]".
+        iDestruct "H" as (a) "[Hf [H _]]".
+        iExists _. iFrame. iSplit =>//.
+        iIntros "Hf".
+        
+        
+        
+      }
+    }
+
+    
+  Lemma wp_seq_trap_ctx (s : stuckness) (E : coPset) (es1 es2 : language.expr wasm_lang) f f' i lh :
+    ↪[frame] f ∗
+     (↪[frame] f -∗ WP es1 @ NotStuck; E {{ w, ⌜w = trapV⌝ ∗ ↪[frame] f' }})
+     ⊢ WP (es1 ++ es2) @ s; E CTX i; lh {{ w, ⌜w = trapV⌝ ∗ ↪[frame] f' }}.
+  Proof.
+    iIntros "[Hf Hes1]".
+    iInduction i as [|i] "IH" forall (E es1 es2 lh f f' s).
+    { iIntros (LI Hfilled).
+      apply lfilled_Ind_Equivalent in Hfilled.
+      inversion Hfilled;subst.
+      erewrite app_assoc.
+      iApply (wp_seq_trap with "[Hf Hes1]"). iFrame.
+      iIntros "Hf".
+      apply const_list_is_val in H as Hv.
+      destruct Hv as [v Hv].
+      iApply (wp_val_app_trap with "[-]");eauto.
+      iFrame. iIntros "Hf".
+      iApply (wp_seq_trap with "[-]");eauto.
+      iFrame. }
+    { iIntros (LI Hfilled).
+      apply lfilled_Ind_Equivalent in Hfilled.
+      inversion Hfilled;subst.
+      iApply (wp_label_trap with "Hf");auto.
+      iIntros "Hf".
+      iDestruct ("IH" $! _ _ _ _ _ _ NotStuck with "Hf Hes1") as "H".
+      apply lfilled_Ind_Equivalent in H1.
+      iSpecialize ("H" $! _ H1). auto.
+    }
+  Qed.
+
+    
+    iLöb as "IH" forall (s E es1 es2 f f').
+    iIntros (LI Hfilled). iApply wp_unfold.
+    repeat rewrite wp_unfold /wp_pre /=.
+    destruct (iris.to_val LI) as [vs|] eqn:Hetov.
+    { destruct vs.
+    { pose proof (filled_is_val_imm _ _ _ _ _ Hetov Hfilled) as
+        [vs [es' [-> [-> [Hconst1 Hconst2]]]]].
+      apply const_list_is_val in Hconst1 as [v1 Hv1].
+      apply const_list_is_val in Hconst2 as [v2 Hv2].
+      edestruct fill_val as [vs12 [Hvs12 Heql]];eauto.
+      assert (Hvs12':=Hvs12).
+      apply to_val_cat in Hvs12' as [-> Hev2].
+      apply iris.of_to_val in Hev2 as <-.
+      iMod ("Hes1" with "Hf") as "[%Hcontr _]". done.
+    }
+    { apply to_val_trap_is_singleton in Hetov. subst.
+      apply lfilled_Ind_Equivalent in Hfilled.
+      inversion Hfilled;subst.
+      2: { exfalso. do 2 destruct vs =>//=. }
+      apply app_eq_singleton in H as [[HH HH']|[HH HH']];subst.
+      { exfalso. destruct es1,es2,es' =>//=. }
+      apply app_eq_singleton in HH' as [[HH HH']|[HH HH']];subst.
+      { apply app_eq_singleton in HH as [[-> ->]|[-> ->]].
+        simpl.
+        all: iMod ("Hes1" with "Hf") as "[%Hcontr Hes2]".
+        auto. done. }
+      { destruct es1,es2 =>//=.
+        iMod ("Hes1" with "[$]") as "[%Hcontr _]";done. }
+    }
+    }
+    (* Ind *)
+    iIntros (σ ns κ κs nt) "Hσ".
+    destruct (iris.to_val es1) as [vs|] eqn:Hes.
+    { apply of_to_val in Hes as <-.
+    iMod ("Hes1" with "Hf") as "[%Heq Hf]". subst.
+    iApply fupd_frame_l.
+    iSplit.
+    { iPureIntro.
+      destruct s =>//.
+      unfold iris_wp_def.reducible, reducible.
+      revert lh LI Hfilled Hetov. induction i =>lh LI Hfilled Hetov.
+      { apply lfilled_Ind_Equivalent in Hfilled.
+        inversion Hfilled;subst.
+        eexists _,[AI_trap],σ,_.
+        destruct σ as [[[? ?]?]?]. simpl.
+        repeat split;eauto.
+        eapply r_simple,rs_trap.
+        2: instantiate (1 := LH_base vs (es2 ++ es'));apply lfilled_Ind_Equivalent;by constructor.
+        destruct vs,es2,es' =>//.
+        1,2,3,4:destruct vs =>//.
+      }
+      { apply lfilled_Ind_Equivalent in Hfilled.
+        inversion Hfilled;subst.
+        destruct (iris.to_val LI0) eqn:Hval.
+        { destruct v.
+          { exfalso. apply lfilled_Ind_Equivalent in H1 as Heq.
+            eapply filled_is_val_imm in Heq;eauto.
+            destruct Heq as [vs' [esn [? [? ?]]]].
+            simplify_eq. inversion H1. simplify_eq.
+            simpl in Hval.
+            destruct vs',es2,esn;try done.
+            all:rewrite to_val_not_trap_interweave in Hval;auto; done. }
+          { apply lfilled_Ind_Equivalent in H1 as Heq.
+            eapply filled_is_val_trap in Heq as [-> ->];eauto.
+            inversion H1;simplify_eq.
+            erewrite app_nil_r in Hval.
+            destruct es2 =>//.
+            repeat erewrite app_nil_l,app_nil_r. rewrite app_nil_r /=.
+            eexists _,(vs++[AI_trap]++es''),σ,_.
+            destruct σ as [[[? ?]?]?]. simpl.
+            repeat split;eauto.
+            repeat erewrite app_nil_l,app_nil_r in Hfilled.
+            erewrite app_nil_r in Hfilled.
+            apply lfilled_Ind_Equivalent in Hfilled.
+            eapply r_label with (es:=[AI_label n es' [AI_trap]]);eauto.
+            2: instantiate (1 := LH_base vs es'');apply lfilled_Ind_Equivalent; by constructor.
+            apply r_simple,rs_label_trap.
+            apply lfilled_Ind_Equivalent. by constructor. }
+        }
+        apply lfilled_Ind_Equivalent in H1.
+        eapply IHi in Hval as [? [? [? [? ?]]]];eauto.
+        destruct σ as [[[? ?]?]?]. simpl in *.
+        assert (lfilled 1 (LH_rec vs n es' (LH_base [] []) es'') LI0 (vs ++ AI_label n es' LI0 :: es'')) as Hfill.
+        { apply lfilled_Ind_Equivalent. constructor;auto.
+          apply lfilled_Ind_Equivalent. cbn.
+          rewrite app_nil_r eqseqE. done. }
+        apply lfilled_swap with (es':=x0) in Hfill as Hfill2.
+        destruct Hfill2 as [LI' HLI'].
+        eexists _,LI',x1,_.
+        destruct x1 as [[[? ?]?]?]. simpl in *.
+        destruct H as [? [-> ->]].
+        repeat split;eauto.
+        eapply r_label. apply r. apply Hfill.
+        apply HLI'.
+      }
+    }
+    { iApply fupd_mask_intro;[solve_ndisj|].
+      iIntros "Hcls".
+      iIntros (e2 σ2 efs Hstep).
+      iModIntro. iNext. iModIntro.
+      iMod "Hcls". iModIntro.
+      
+      destruct σ as [[[? ?]?]?].
+      destruct σ2 as [[[? ?]?]?].
+      simpl in *. destruct Hstep as [Hstep [-> ->]].
+      iInduction i as [|j IHj] "IHj".
+      { apply lfilled_Ind_Equivalent in Hfilled.
+        inversion Hfilled;subst.
+        assert (lfilled 0 (LH_base vs (es2 ++ es')) [AI_trap] (vs ++ of_val trapV ++ es2 ++ es')) as Hfill.
+        { apply lfilled_Ind_Equivalent. constructor. done. }
+        eapply trap_reduce in Hstep as Hred;[|apply Hfill].
+        destruct Hred as [lh' [Hfill' Heq]]. simplify_eq.
+        apply lfilled_Ind_Equivalent in Hfill'. inversion Hfill';subst.
+        iApply bi.sep_exist_l. iExists _. iFrame. iSplit =>//.
+        iIntros "Hf".
+        iApply wp_trap;eauto. }
+      { }
+
+        erewrite app_assoc.
+        iApply ("IH" with "[$Hf]").
+        iIntros "Hf".
+        iApply wp_trap;eauto. iPureIntro. }
+
+
+      
+      eapply trap_reduce in Hstep as Hred;[|apply Hfill].
+      destruct Hred as [lh' [Hfill' Heq]]. simplify_eq.
+      apply lfilled_Ind_Equivalent in Hfill'. inversion Hfill';subst.
+      iApply bi.sep_exist_l. iExists _. iFrame. iSplit =>//.
+      iIntros "Hf". erewrite app_assoc.
+      iApply ("IH" with "[$Hf]").
+      iIntros "Hf".
+      iApply wp_trap;eauto. }
+    }
+
+
+
+
+
+    
+  { destruct σ as [[[? ?]?]?].
+    set (σ:=(s0,s1,l,i)).
+    iDestruct "Hσ" as "(?&?&?&?&Hfr&?)".
+    iDestruct (ghost_map_lookup with "Hfr Hf") as %Heq1.
+    iSpecialize ("Hes1" with "[$]").
+    iSpecialize ("Hes1" $! σ ns κ κs nt with "[$]").
+    iMod "Hes1" as "[%H1 H2]".
+    iModIntro.
+    iSplit.
+    - iPureIntro.
+      destruct s => //.
+      by apply append_reducible.
+    - iIntros (e2 σ2 efs HStep).
+      assert (κ = [] /\ efs = []) as [-> ->]; first by apply prim_step_obs_efs_empty in HStep; inversion HStep.
+      apply prim_step_split_reduce_r in HStep; last by [].
+      destruct HStep as [[es'' [-> HStep]] | [n [m [lh [Hlf1 [Hlf2 ->]]]]]].
+      + iSpecialize ("H2" $! es'' σ2 [] HStep).
+        iMod "H2".
+        repeat iModIntro.
+        repeat iMod "H2".
+        iModIntro.
+        destruct σ2 as [[[??] ?]?].
+        iDestruct "H2" as "[Hσ H]".
+        iDestruct "H" as (f1) "(Hf1 & Hes'' & Hefs)".
+        iApply bi.sep_exist_l. iExists f1.
+        iFrame. (* iSplit =>//. *)
+        iIntros "?".
+        iSpecialize ("IH" with "[$]").
+        iApply "IH". eauto.
+      + move/lfilledP in Hlf1.
+        inversion Hlf1; subst; clear Hlf1.
+        assert (iris.prim_step es1 σ [] [AI_trap] σ []) as HStep2.
+        { unfold iris.prim_step.
+          destruct σ as [[[??]?]?].
+          repeat split => //.
+          apply r_simple; eapply rs_trap => //.
+          move => HContra; subst.
+          by destruct n.
+        }
+        iSpecialize ("H2" $! [AI_trap] σ [] HStep2).
+        iMod "H2".
+        repeat iModIntro.
+        repeat iMod "H2".
+        destruct σ as [[[??] ?]?].
+        iDestruct "H2" as "[Hσ H]".
+        iDestruct "H" as (f1) "(Hf1 & Hes'' & Hefs)".
+        iApply bi.sep_exist_l.  iExists f1.
+        iDestruct "Hσ" as "(?&?&?&?&Hfr&?)".
+        iDestruct (ghost_map_lookup with "Hfr Hf1") as %Heq.
+        iDestruct ("Hes''" with "Hf1") as "Hes''".
+        rewrite wp_unfold /wp_pre /=.
+        iMod "Hes''" as "[_ Hf1]".
+        iDestruct (ghost_map_lookup with "Hfr Hf1") as %Heq'.
+        simplify_map_eq.
+        (* iModIntro. *)
+        iFrame. (* iApply fupd_frame_r. iSplit =>//. *)
+        iModIntro. iIntros "Hf".
+        erewrite cons_middle.
+        erewrite app_assoc.
+        iApply ("IH" with "[$Hf]").
+        iIntros "Hf".
+        iApply wp_trap;auto. }
+  Qed.
+
+  
+
+  Lemma wp_seq_trap_or (s : stuckness) (E : coPset) (Φ Ψ : val -> iProp Σ) (es1 es2 : language.expr wasm_lang) f :
+    (↪[frame] f ∗ (¬ (Ψ trapV)) ∗
+     (↪[frame] f -∗ WP es1 @ s; E {{ w, (⌜w = trapV⌝ ∨ Ψ w) ∗ ∃ f', ↪[frame] f' }}) ∗
+     ∀ w f', Ψ w ∗ ↪[frame] f' -∗ WP (iris.of_val w ++ es2) @ s; E {{ v, Φ v ∗ ∃ f', ↪[frame] f' }})%I
+     ⊢ WP (es1 ++ es2) @ s; E {{ w, (⌜w = trapV⌝ ∨ Ψ w) ∗ ∃ f', ↪[frame] f' }}.
+
+
+    Proof.
+    iIntros "(Hf & Htrap & Hcont)".
+    
   
 End trap_rules.
